Exploring consequences on components of new definitions.

Dynamical_Systems.thy
@@ -128,44 +128,6 @@ lemma "\<nu> \<in> g_orbital f G (\<lambda>s. {t. t \<ge> 0}) 0 \<omega> \<longl
 
 no_notation g_orbit ("\<gamma>")
 
-subsection \<open> Verification components \<close>
-
-type_synonym 'a pred = "'a \<Rightarrow> bool"
-type_synonym 's prog = "'s \<Rightarrow> 's set"
-
-definition fbox :: "('a \<Rightarrow> 'b set) \<Rightarrow> 'b pred \<Rightarrow> 'a pred" ("|_] _" [61,81] 82)
-  where "|F] P = (\<lambda>s. (\<forall>s'. s' \<in> F s \<longrightarrow> P s'))"
-
-lemma fbox_iso: "P \<le> Q \<Longrightarrow> |F] P \<le> |F] Q"
-  unfolding fbox_def by auto
-
-lemma fbox_anti: "\<forall>s. F\<^sub>1 s \<subseteq> F\<^sub>2 s \<Longrightarrow> |F\<^sub>2] P \<le> |F\<^sub>1] P"
-  unfolding fbox_def by auto
-
-lemma fbox_invariants: 
-  assumes "I \<le> |F] I" and "J \<le> |F] J"
-  shows "(\<lambda>s. I s \<and> J s) \<le> |F] (\<lambda>s. I s \<and> J s)"
-    and "(\<lambda>s. I s \<or> J s) \<le> |F] (\<lambda>s. I s \<or> J s)"
-  using assms unfolding fbox_def by auto
-
-subsection \<open> Verification of hybrid programs \<close>
-
-text \<open> Verification by providing evolution \<close>
-
-definition g_evol :: "(('a::real_vector) \<Rightarrow> 'b \<Rightarrow> 'b) \<Rightarrow> 'b pred \<Rightarrow> ('b \<Rightarrow> 'a set) \<Rightarrow> ('b \<Rightarrow> 'b set)" ("EVOL")
-  where "EVOL \<phi> G U = (\<lambda>s. g_orbit G (U s) 0 (\<lambda>t. \<phi> t s))"
-
-lemma fbox_g_evol[simp]: 
-  fixes \<phi> :: "('a::real_vector) \<Rightarrow> 'b \<Rightarrow> 'b"
-  shows "|EVOL \<phi> G U] Q = (\<lambda>s. (\<forall>t\<in>U s. (\<forall>\<tau>\<in>{0--t}. G (\<phi> \<tau> s)) \<longrightarrow> Q (\<phi> t s)))"
-  unfolding g_evol_def g_orbit_def fbox_def by auto
-
-text \<open> Verification by providing solutions \<close>
-
-lemma fbox_g_orbital: "|g_orbital f G U t\<^sub>0] Q = 
-  (\<lambda>s. \<forall>t. \<forall>X\<in>Sols f {t\<^sub>0--t} t\<^sub>0 s. {t\<^sub>0--t} \<subseteq> U s \<longrightarrow> (\<forall>\<tau>\<in>{t\<^sub>0--t}. G (X \<tau>)) \<longrightarrow> Q (X t))"
-  unfolding fbox_def g_orbital_eq by (auto simp: fun_eq_iff)
-
 
 subsection \<open> Differential Invariants \<close>
 
@@ -227,7 +189,7 @@ qed
 
 named_theorems diff_inv_rules "rules for certifying differential invariants"
 
-lemma diff_inv_eq_zero:
+lemma diff_inv_eq0I:
   fixes \<mu>::"'a::real_normed_vector \<Rightarrow> 'b::real_inner"
   assumes "\<And>X t. {t\<^sub>0--t} \<subseteq> U (X t\<^sub>0) \<Longrightarrow> (D X = (\<lambda>\<tau>. f \<tau> (X \<tau>)) on {t\<^sub>0--t}) \<Longrightarrow> \<forall>\<tau>\<in>{t\<^sub>0--t}. G (X \<tau>) \<Longrightarrow> 
     D (\<lambda>\<tau>. \<mu> (X \<tau>)) = (\<lambda>\<tau>. \<tau> *\<^sub>R 0) on {t\<^sub>0--t}"
@@ -248,22 +210,23 @@ proof(clarsimp simp: diff_inv_eq ivp_sols_def)
     using xivp by auto
 qed
 
-lemma diff_inv_eq_rule [diff_inv_rules]:
+lemma diff_inv_eqI [diff_inv_rules]:
   fixes \<mu>::"'a::real_normed_vector \<Rightarrow> 'b::real_inner"
   assumes "\<And>X t. {t\<^sub>0--t} \<subseteq> U (X t\<^sub>0) \<Longrightarrow> (D X = (\<lambda>\<tau>. f \<tau> (X \<tau>)) on {t\<^sub>0--t}) \<Longrightarrow> \<forall>\<tau>\<in>{t\<^sub>0--t}. G (X \<tau>) \<Longrightarrow> 
     D (\<lambda>\<tau>. \<mu> (X \<tau>) - \<nu> (X \<tau>)) = (\<lambda>\<tau>. \<tau> *\<^sub>R 0) on {t\<^sub>0--t}"
   shows "diff_inv (\<lambda>s. \<mu> s = \<nu> s) f U t\<^sub>0 G"
-  using diff_inv_eq_zero[where \<mu>="\<lambda>s. \<mu> s - \<nu> s"] assms by auto
+  using diff_inv_eq0I[where \<mu>="\<lambda>s. \<mu> s - \<nu> s"] assms by auto
 
 text \<open> can this be generalised to @{term "\<mu>::'a::real_normed_vector \<Rightarrow> 'b::real_inner"}? \<close>
-lemma diff_inv_leq_rule [diff_inv_rules]:
+lemma 
   fixes \<mu>::"'a::real_normed_vector \<Rightarrow> real"
   assumes "\<And>X t. {t\<^sub>0--t} \<subseteq> U (X t\<^sub>0) \<Longrightarrow> (D X = (\<lambda>\<tau>. f \<tau> (X \<tau>)) on {t\<^sub>0--t}) \<Longrightarrow> \<forall>\<tau>\<in>{t\<^sub>0--t}. G (X \<tau>) \<Longrightarrow> 
     (D (\<lambda>\<tau>. \<mu> (X \<tau>)) = (\<lambda>\<tau>. \<mu>' (X \<tau>)) on {t\<^sub>0--t}) \<and> (\<forall>\<tau>\<in>{t\<^sub>0<--<t}. (\<tau> > t\<^sub>0 \<longrightarrow> \<mu>' (X \<tau>) \<ge> 0) \<and> (\<tau> < t\<^sub>0 \<longrightarrow> \<mu>' (X \<tau>) \<le> 0))"
-  shows "diff_inv (\<lambda>s. 0 < \<mu> s) f U t\<^sub>0 G"
-proof(clarsimp simp: diff_inv_eq ivp_sols_def)
+  shows diff_inv_leq0I: "diff_inv (\<lambda>s. 0 \<le> \<mu> s) f U t\<^sub>0 G"
+    and diff_inv_less0I: "diff_inv (\<lambda>s. 0 < \<mu> s) f U t\<^sub>0 G"
+proof(auto simp: diff_inv_eq ivp_sols_def)
   fix X t
-  assume xivp: "D X = (\<lambda>\<tau>. f \<tau> (X \<tau>)) on {t\<^sub>0--t}" "0 < \<mu> (X t\<^sub>0)"
+  assume xivp: "D X = (\<lambda>\<tau>. f \<tau> (X \<tau>)) on {t\<^sub>0--t}"
     and ghyp: "\<forall>\<tau>\<in>{t\<^sub>0--t}. G (X \<tau>)" and ivl: "{t\<^sub>0--t} \<subseteq> U (X t\<^sub>0)"
   hence key: "D (\<lambda>\<tau>. \<mu> (X \<tau>)) = (\<lambda>\<tau>. \<mu>' (X \<tau>)) on {t\<^sub>0--t}"
     using assms by auto
@@ -274,12 +237,13 @@ proof(clarsimp simp: diff_inv_eq ivp_sols_def)
       unfolding open_segment_eq_real_ivl by auto
     hence "t\<^sub>0 < t \<Longrightarrow> 0 \<le> \<mu>' (X \<tau>)" and "t < t\<^sub>0 \<Longrightarrow> \<mu>' (X \<tau>) \<le> 0"
       using assms[OF ivl xivp(1) ghyp] \<open>\<tau> \<in> {t\<^sub>0<--<t}\<close> by auto
-    hence "\<mu> (X t) > 0"
-      using mvt xivp(2) \<open>t\<^sub>0 \<noteq> t\<close> mult_nonneg_nonneg mult_neg_neg
+    hence "(0 < \<mu> (X t\<^sub>0) \<longrightarrow> \<mu> (X t) > 0) \<and> (0 \<le> \<mu> (X t\<^sub>0) \<longrightarrow> 0 \<le> \<mu> (X t))"
+      using mvt \<open>t\<^sub>0 \<noteq> t\<close> mult_nonneg_nonneg mult_neg_neg
       by (metis add_nonneg_nonneg diff_gt_0_iff_gt le_add_same_cancel2 
           less_eq_real_def linorder_not_le mult_eq_0_iff)}
-  thus "0 < \<mu> (X t)"
-    using xivp(2) by blast
+  thus "0 < \<mu> (X t\<^sub>0) \<Longrightarrow> 0 < \<mu> (X t)" 
+    and "0 \<le> \<mu> (X t\<^sub>0) \<Longrightarrow> 0 \<le> \<mu> (X t)"
+    by blast+
 qed
 
 lemma 
@@ -287,173 +251,518 @@ lemma
   assumes "\<And>X t. {t\<^sub>0--t} \<subseteq> U (X t\<^sub>0) \<Longrightarrow> (D X = (\<lambda>\<tau>. f \<tau> (X \<tau>)) on {t\<^sub>0--t}) \<Longrightarrow> \<forall>\<tau>\<in>{t\<^sub>0--t}. G (X \<tau>) \<Longrightarrow> 
     (D (\<lambda>\<tau>. \<mu>(X \<tau>)-\<nu>(X \<tau>)) = (\<lambda>\<tau>. \<mu>'(X \<tau>)-\<nu>'(X \<tau>)) on {t\<^sub>0--t}) \<and> 
     (\<forall>\<tau>\<in>{t\<^sub>0<--<t}. (\<tau> > t\<^sub>0 \<longrightarrow> \<mu>' (X \<tau>) \<ge> \<nu>' (X \<tau>)) \<and> (\<tau> < t\<^sub>0 \<longrightarrow> \<mu>' (X \<tau>) \<le> \<nu>' (X \<tau>)))"
-  shows "diff_inv (\<lambda>s. \<nu> s < \<mu> s) f U t\<^sub>0 G"
-  apply(subgoal_tac "diff_inv (\<lambda>s. \<nu> s < \<mu> s) f U t\<^sub>0 G = diff_inv (\<lambda>s. 0 < \<mu> s - \<nu> s) f U t\<^sub>0 G")
-  using diff_inv_leq_rule[where \<mu>="\<lambda>s. \<mu> s - \<nu> s" and \<mu>'="\<lambda>s. \<mu>' s - \<nu>' s"] assms
-   apply auto[1]
-  apply(rule arg_cong[where f="\<lambda>P. diff_inv P f U t\<^sub>0 G"])
-  by auto (* HERE *)
+  shows diff_inv_leqI [diff_inv_rules]: "diff_inv (\<lambda>s. \<nu> s \<le> \<mu> s) f U t\<^sub>0 G"
+    and diff_inv_lessI [diff_inv_rules]: "diff_inv (\<lambda>s. \<nu> s < \<mu> s) f U t\<^sub>0 G"
+  using diff_inv_less0I[where \<mu>="\<lambda>s. \<mu> s - \<nu> s" and \<mu>'="\<lambda>s. \<mu>' s - \<nu>' s"] assms 
+  diff_inv_leq0I[where \<mu>="\<lambda>s. \<mu> s - \<nu> s" and \<mu>'="\<lambda>s. \<mu>' s - \<nu>' s"] by auto
 
-
-
-lemma diff_inv_leq_rule [diff_inv_rules]:
+lemma diff_inv_nleq_iff:
   fixes \<mu>::"'a::banach \<Rightarrow> real"
-  assumes Gg: "\<And>X t. (D X = (\<lambda>\<tau>. f \<tau> (X \<tau>)) on {t\<^sub>0--t}) \<Longrightarrow> (\<forall>\<tau>\<in>U(X t\<^sub>0). \<tau> > t\<^sub>0 \<longrightarrow> G (X \<tau>) \<longrightarrow> \<mu>' (X \<tau>) \<ge> \<nu>' (X \<tau>))"
-    and Gl: "\<And>X. (D X = (\<lambda>\<tau>. f \<tau> (X \<tau>)) on U(X t\<^sub>0)) \<Longrightarrow> (\<forall>\<tau>\<in>U(X t\<^sub>0). \<tau> < t\<^sub>0 \<longrightarrow> \<mu>' (X \<tau>) \<le> \<nu>' (X \<tau>))"
-    and dX: "\<And>X. (D X = (\<lambda>\<tau>. f \<tau> (X \<tau>)) on U(X t\<^sub>0)) \<Longrightarrow> D (\<lambda>\<tau>. \<mu>(X \<tau>)-\<nu>(X \<tau>)) = (\<lambda>\<tau>. \<mu>'(X \<tau>)-\<nu>'(X \<tau>)) on U(X t\<^sub>0)"
-  shows "diff_inv (\<lambda>s. \<nu> s \<le> \<mu> s) f U t\<^sub>0 G"
-proof(simp_all add: diff_inv_eq ivp_sols_def, safe)
-  fix X t assume Ghyp: "\<forall>\<tau>. \<tau> \<in> U (X t\<^sub>0) \<and> \<tau> \<le> t \<longrightarrow> G (X \<tau>)"
-  assume xivp: "D X = (\<lambda>x. f x (X x)) on U (X t\<^sub>0)" "\<nu> (X t\<^sub>0) \<le> \<mu> (X t\<^sub>0)" "X \<in> U (X t\<^sub>0) \<rightarrow> S"
-  assume tHyp: "t \<in> U (X t\<^sub>0)" and t0Hyp: "t\<^sub>0 \<in> U (X t\<^sub>0)" 
-  hence obs1: "{t\<^sub>0--t} \<subseteq> U (X t\<^sub>0)" "{t\<^sub>0<--<t} \<subseteq> U (X t\<^sub>0)"
-    using closed_segment_subset_interval[OF Uhyp t0Hyp tHyp] xivp(3) segment_open_subset_closed
-    by (force, metis PiE \<open>X t\<^sub>0 \<in> S \<Longrightarrow> {t\<^sub>0--t} \<subseteq> U (X t\<^sub>0)\<close> dual_order.trans)
-  hence obs2: "D (\<lambda>\<tau>. \<mu> (X \<tau>) - \<nu> (X \<tau>)) = (\<lambda>\<tau>. \<mu>' (X \<tau>) - \<nu>' (X \<tau>)) on {t\<^sub>0--t}"
-    using has_vderiv_on_subset[OF dX[OF xivp(1)]] by auto
-  {assume "t \<noteq> t\<^sub>0"
-    then obtain r where rHyp: "r \<in> {t\<^sub>0<--<t}" 
-      and "(\<mu>(X t)-\<nu>(X t)) - (\<mu>(X t\<^sub>0)-\<nu>(X t\<^sub>0)) = (\<lambda>\<tau>. \<tau>*(\<mu>'(X r)-\<nu>'(X r))) (t - t\<^sub>0)"
-      using mvt_simple_closed_segmentE obs2 by blast
-    hence mvt: "\<mu>(X t)-\<nu>(X t) = (t - t\<^sub>0)*(\<mu>'(X r)-\<nu>'(X r)) + (\<mu>(X t\<^sub>0)-\<nu>(X t\<^sub>0))"
-      by force
-    have primed: "\<And>\<tau>. \<tau> \<in> U (X t\<^sub>0) \<Longrightarrow> \<tau> > t\<^sub>0 \<Longrightarrow> G (X \<tau>) \<Longrightarrow> \<mu>' (X \<tau>) \<ge> \<nu>' (X \<tau>)" 
-      "\<And>\<tau>. \<tau> \<in> U (X t\<^sub>0) \<Longrightarrow> \<tau> < t\<^sub>0 \<Longrightarrow> \<mu>' (X \<tau>) \<le> \<nu>' (X \<tau>)"
-      using Gg[OF xivp(1)] Gl[OF xivp(1)] by auto
-    have "t > t\<^sub>0 \<Longrightarrow> r > t\<^sub>0 \<and> G (X r)" "\<not> t\<^sub>0 \<le> t \<Longrightarrow> r < t\<^sub>0" "r \<in> U (X t\<^sub>0)"
-      using \<open>r \<in> {t\<^sub>0<--<t}\<close> obs1 Ghyp
-      unfolding open_segment_eq_real_ivl closed_segment_eq_real_ivl by auto
-    moreover have "r > t\<^sub>0 \<Longrightarrow> G (X r) \<Longrightarrow> (\<mu>'(X r)- \<nu>'(X r)) \<ge> 0" "r < t\<^sub>0 \<Longrightarrow> (\<mu>'(X r)-\<nu>'(X r)) \<le> 0"
-      using primed(1,2)[OF \<open>r \<in> U (X t\<^sub>0)\<close>] by auto
-    ultimately have "(t - t\<^sub>0) * (\<mu>'(X r)-\<nu>'(X r)) \<ge> 0"
-      by (case_tac "t \<ge> t\<^sub>0", force, auto simp: split_mult_pos_le)
-    hence "(t - t\<^sub>0) * (\<mu>'(X r)-\<nu>'(X r)) + (\<mu>(X t\<^sub>0)-\<nu>(X t\<^sub>0)) \<ge> 0"
-      using xivp(2) by auto
-    hence "\<nu> (X t) \<le> \<mu> (X t)"
-      using mvt by simp}
-  thus "\<nu> (X t) \<le> \<mu> (X t)"
-    using xivp by blast
-qed
+  shows "diff_inv (\<lambda>s. \<not> \<nu> s \<le> \<mu> s) f U t\<^sub>0 G \<longleftrightarrow> diff_inv (\<lambda>s. \<nu> s > \<mu> s) f U t\<^sub>0 G"
+  unfolding diff_inv_eq approximation_preproc_push_neg(2) by presburger
 
-lemma diff_inv_less_rule [diff_inv_rules]:
+lemma diff_inv_neqI [diff_inv_rules]:
   fixes \<mu>::"'a::banach \<Rightarrow> real"
-  assumes Uhyp: "\<And>s. s \<in> S \<Longrightarrow> is_interval (U s)"
-    and Gg: "\<And>X. (D X = (\<lambda>\<tau>. f \<tau> (X \<tau>)) on U(X t\<^sub>0)) \<Longrightarrow> (\<forall>\<tau>\<in>U(X t\<^sub>0). \<tau> > t\<^sub>0 \<longrightarrow> G (X \<tau>) \<longrightarrow> \<mu>' (X \<tau>) \<ge> \<nu>' (X \<tau>))"
-    and Gl: "\<And>X. (D X = (\<lambda>\<tau>. f \<tau> (X \<tau>)) on U(X t\<^sub>0)) \<Longrightarrow> (\<forall>\<tau>\<in>U(X t\<^sub>0). \<tau> < t\<^sub>0 \<longrightarrow> \<mu>' (X \<tau>) \<le> \<nu>' (X \<tau>))"
-    and dX: "\<And>X. (D X = (\<lambda>\<tau>. f \<tau> (X \<tau>)) on U(X t\<^sub>0)) \<Longrightarrow> D (\<lambda>\<tau>. \<mu>(X \<tau>)-\<nu>(X \<tau>)) = (\<lambda>\<tau>. \<mu>'(X \<tau>)-\<nu>'(X \<tau>)) on U(X t\<^sub>0)"
-  shows "diff_inv (\<lambda>s. \<nu> s < \<mu> s) f U S t\<^sub>0 G"
-proof(simp_all add: diff_inv_eq ivp_sols_def, safe)
-  fix X t assume Ghyp: "\<forall>\<tau>. \<tau> \<in> U (X t\<^sub>0) \<and> \<tau> \<le> t \<longrightarrow> G (X \<tau>)"
-  assume xivp: "D X = (\<lambda>x. f x (X x)) on U (X t\<^sub>0)" "\<nu> (X t\<^sub>0) < \<mu> (X t\<^sub>0)" "X \<in> U (X t\<^sub>0) \<rightarrow> S"
-  assume tHyp: "t \<in> U (X t\<^sub>0)" and t0Hyp: "t\<^sub>0 \<in> U (X t\<^sub>0)" 
-  hence obs1: "{t\<^sub>0--t} \<subseteq> U (X t\<^sub>0)" "{t\<^sub>0<--<t} \<subseteq> U (X t\<^sub>0)"
-    using closed_segment_subset_interval[OF Uhyp t0Hyp tHyp] xivp(3) segment_open_subset_closed
-    by (force, metis PiE \<open>X t\<^sub>0 \<in> S \<Longrightarrow> {t\<^sub>0--t} \<subseteq> U (X t\<^sub>0)\<close> dual_order.trans)
-  hence obs2: "D (\<lambda>\<tau>. \<mu> (X \<tau>) - \<nu> (X \<tau>)) = (\<lambda>\<tau>. \<mu>' (X \<tau>) - \<nu>' (X \<tau>)) on {t\<^sub>0--t}"
-    using has_vderiv_on_subset[OF dX[OF xivp(1)]] by auto
-  {assume "t \<noteq> t\<^sub>0"
-    then obtain r where rHyp: "r \<in> {t\<^sub>0<--<t}" 
-      and "(\<mu>(X t)-\<nu>(X t)) - (\<mu>(X t\<^sub>0)-\<nu>(X t\<^sub>0)) = (\<lambda>\<tau>. \<tau>*(\<mu>'(X r)-\<nu>'(X r))) (t - t\<^sub>0)"
-      using mvt_simple_closed_segmentE obs2 by blast
-    hence mvt: "\<mu>(X t)-\<nu>(X t) = (t - t\<^sub>0)*(\<mu>'(X r)-\<nu>'(X r)) + (\<mu>(X t\<^sub>0)-\<nu>(X t\<^sub>0))"
-      by force
-    have primed: "\<And>\<tau>. \<tau> \<in> U (X t\<^sub>0) \<Longrightarrow> \<tau> > t\<^sub>0 \<Longrightarrow> G (X \<tau>) \<Longrightarrow> \<mu>' (X \<tau>) \<ge> \<nu>' (X \<tau>)" 
-      "\<And>\<tau>. \<tau> \<in> U (X t\<^sub>0) \<Longrightarrow> \<tau> < t\<^sub>0 \<Longrightarrow> \<mu>' (X \<tau>) \<le> \<nu>' (X \<tau>)"
-      using Gg[OF xivp(1)] Gl[OF xivp(1)] by auto
-    have "t > t\<^sub>0 \<Longrightarrow> r > t\<^sub>0 \<and> G (X r)" "\<not> t\<^sub>0 \<le> t \<Longrightarrow> r < t\<^sub>0" "r \<in> U (X t\<^sub>0)"
-      using \<open>r \<in> {t\<^sub>0<--<t}\<close> obs1 Ghyp
-      unfolding open_segment_eq_real_ivl closed_segment_eq_real_ivl by auto
-    moreover have "r > t\<^sub>0 \<Longrightarrow> G (X r) \<Longrightarrow> (\<mu>'(X r)- \<nu>'(X r)) \<ge> 0" "r < t\<^sub>0 \<Longrightarrow> (\<mu>'(X r)-\<nu>'(X r)) \<le> 0"
-      using primed(1,2)[OF \<open>r \<in> U (X t\<^sub>0)\<close>] by auto
-    ultimately have "(t - t\<^sub>0) * (\<mu>'(X r)-\<nu>'(X r)) \<ge> 0"
-      by (case_tac "t \<ge> t\<^sub>0", force, auto simp: split_mult_pos_le)
-    hence "(t - t\<^sub>0) * (\<mu>'(X r)-\<nu>'(X r)) + (\<mu>(X t\<^sub>0)-\<nu>(X t\<^sub>0)) > 0"
-      using xivp(2) by auto
-    hence "\<nu> (X t) < \<mu> (X t)"
-      using mvt by simp}
-  thus "\<nu> (X t) < \<mu> (X t)"
-    using xivp by blast
-qed
-
-lemma diff_inv_nleq_rule:
-  fixes \<mu>::"'a::banach \<Rightarrow> real"
-  shows "diff_inv (\<lambda>s. \<not> \<nu> s \<le> \<mu> s) f U S t\<^sub>0 G \<longleftrightarrow> diff_inv (\<lambda>s. \<nu> s > \<mu> s) f U S t\<^sub>0 G"
-  unfolding diff_inv_eq apply safe
-  by (clarsimp, erule_tac x=s in allE, simp, erule_tac x=X in ballE, force, force)+
-
-lemma diff_inv_neq_rule [diff_inv_rules]:
-  fixes \<mu>::"'a::banach \<Rightarrow> real"
-  assumes "diff_inv (\<lambda>s. \<nu> s < \<mu> s) f U S t\<^sub>0 G"
-    and "diff_inv (\<lambda>s. \<nu> s > \<mu> s) f U S t\<^sub>0 G"
-  shows "diff_inv (\<lambda>s. \<nu> s \<noteq> \<mu> s) f U S t\<^sub>0 G"
+  assumes "diff_inv (\<lambda>s. \<nu> s < \<mu> s) f U t\<^sub>0 G"
+    and "diff_inv (\<lambda>s. \<nu> s > \<mu> s) f U t\<^sub>0 G"
+  shows "diff_inv (\<lambda>s. \<nu> s \<noteq> \<mu> s) f U t\<^sub>0 G"
 proof(unfold diff_inv_eq, clarsimp)
   fix s::'a and X::"real \<Rightarrow> 'a" and t::real
-  assume "\<nu> s \<noteq> \<mu> s" and Xhyp: "X \<in> Sols f U S t\<^sub>0 s" 
-     and thyp: "t \<in> U s" and Ghyp: "\<forall>\<tau>. \<tau> \<in> U s \<and> \<tau> \<le> t \<longrightarrow> G (X \<tau>)"
+  assume "\<nu> s \<noteq> \<mu> s" and Xhyp: "X \<in> Sols f {t\<^sub>0--t} t\<^sub>0 s" 
+     and thyp: "{t\<^sub>0--t} \<subseteq> U s" and Ghyp: "\<forall>\<tau>\<in>{t\<^sub>0--t}. G (X \<tau>)"
   hence "\<nu> s < \<mu> s \<or> \<nu> s > \<mu> s"
     by linarith
   moreover have "\<nu> s < \<mu> s \<Longrightarrow> \<nu> (X t) < \<mu> (X t)"
-    using assms(1) Xhyp thyp Ghyp unfolding diff_inv_eq by auto
+    using assms(1) Xhyp thyp Ghyp 
+    unfolding diff_inv_eq by auto
   moreover have "\<nu> s > \<mu> s \<Longrightarrow> \<nu> (X t) > \<mu> (X t)"
-    using assms(2) Xhyp thyp Ghyp unfolding diff_inv_eq by auto
+    using assms(2) Xhyp thyp Ghyp 
+    unfolding diff_inv_eq by auto
   ultimately show "\<nu> (X t) = \<mu> (X t) \<Longrightarrow> False"
     by auto
 qed
 
-lemma diff_inv_neq_rule_converse:
+lemma diff_inv_neqE:
   fixes \<mu>::"'a::banach \<Rightarrow> real"
   assumes Uhyp: "\<And>s. s \<in> S \<Longrightarrow> is_interval (U s)" "\<And>s t. s \<in> S \<Longrightarrow> t \<in> U s \<Longrightarrow> t\<^sub>0 \<le> t"
-    and conts: "\<And>X. (D X = (\<lambda>\<tau>. f \<tau> (X \<tau>)) on U(X t\<^sub>0)) \<Longrightarrow> continuous_on (\<P> X (U (X t\<^sub>0))) \<nu>"
-      "\<And>X. (D X = (\<lambda>\<tau>. f \<tau> (X \<tau>)) on U(X t\<^sub>0)) \<Longrightarrow> continuous_on (\<P> X (U (X t\<^sub>0))) \<mu>"
-    and dI:"diff_inv (\<lambda>s. \<nu> s \<noteq> \<mu> s) f U S t\<^sub>0 G"
-  shows "diff_inv (\<lambda>s. \<nu> s < \<mu> s) f U S t\<^sub>0 G"
+    and conts: "\<And>X t. (D X = (\<lambda>\<tau>. f \<tau> (X \<tau>)) on {t\<^sub>0--t}) \<Longrightarrow> continuous_on (\<P> X {t\<^sub>0--t}) \<nu>"
+      "\<And>X t. (D X = (\<lambda>\<tau>. f \<tau> (X \<tau>)) on {t\<^sub>0--t}) \<Longrightarrow> continuous_on (\<P> X {t\<^sub>0--t}) \<mu>"
+    and dI:"diff_inv (\<lambda>s. \<nu> s \<noteq> \<mu> s) f U t\<^sub>0 G"
+  shows "diff_inv (\<lambda>s. \<nu> s < \<mu> s) f U t\<^sub>0 G"
 proof(unfold diff_inv_eq ivp_sols_def, clarsimp)
-  fix X t assume Ghyp: "\<forall>\<tau>. \<tau> \<in> U (X t\<^sub>0) \<and> \<tau> \<le> t \<longrightarrow> G (X \<tau>)"
-  assume xivp: "D X = (\<lambda>x. f x (X x)) on U (X t\<^sub>0)" "\<nu> (X t\<^sub>0) < \<mu> (X t\<^sub>0)" "X \<in> U (X t\<^sub>0) \<rightarrow> S"
-  assume tHyp: "t \<in> U (X t\<^sub>0)" and t0Hyp: "t\<^sub>0 \<in> U (X t\<^sub>0)"
-  hence "t\<^sub>0 \<le> t" and "\<mu> (X t) \<noteq> \<nu> (X t)"
-    using xivp(3) Uhyp(2) apply force
-    using dI tHyp xivp(2) Ghyp ivp_solsI[of X f U "X t\<^sub>0", OF xivp(1) _ xivp(3) t0Hyp]
-    unfolding diff_inv_eq by force
+  fix X t
+  assume xivp: "D X = (\<lambda>\<tau>. f \<tau> (X \<tau>)) on {t\<^sub>0--t}" "\<nu> (X t\<^sub>0) < \<mu> (X t\<^sub>0)"
+  assume ivl: "{t\<^sub>0--t} \<subseteq> U (X t\<^sub>0)" and Ghyp: "\<forall>\<tau>\<in>{t\<^sub>0--t}. G (X \<tau>)"
+  hence "\<mu> (X t) \<noteq> \<nu> (X t)"
+    using dI xivp ivp_solsI[of X f, OF _ _ ends_in_segment(1)[of t\<^sub>0 t]]
+    unfolding diff_inv_eq by (metis order_less_irrefl)
   moreover
   {assume ineq2:"\<nu> (X t) > \<mu> (X t)"
     note continuous_on_compose[OF vderiv_on_continuous_on[OF xivp(1)]]
-    hence "continuous_on (U (X t\<^sub>0)) (\<nu> \<circ> X)" and "continuous_on (U (X t\<^sub>0)) (\<mu> \<circ> X)"
-      using xivp(1) conts by blast+
-    also have "{t\<^sub>0--t} \<subseteq> U (X t\<^sub>0)"
-      using closed_segment_subset_interval[OF Uhyp(1) t0Hyp tHyp] xivp(3) t0Hyp by auto
-    ultimately have "continuous_on {t\<^sub>0--t} (\<lambda>\<tau>. \<nu> (X \<tau>))" 
+    hence "continuous_on {t\<^sub>0--t} (\<lambda>\<tau>. \<nu> (X \<tau>))" 
       and "continuous_on {t\<^sub>0--t} (\<lambda>\<tau>. \<mu> (X \<tau>))"
-      using continuous_on_subset by auto
+      using xivp(1) conts by force+
     then obtain \<tau> where "\<tau> \<in> {t\<^sub>0--t}" "\<mu> (X \<tau>) = \<nu> (X \<tau>)"
       using IVT_two_functions_real_ivl[OF _ _ xivp(2) ineq2] by force
-    hence "\<forall>r\<in>down (U (X t\<^sub>0)) \<tau>. G (X r)" and "\<tau> \<in> U (X t\<^sub>0)"
-      using Ghyp \<open>\<tau> \<in> {t\<^sub>0--t}\<close> \<open>t\<^sub>0 \<le> t\<close> \<open>{t\<^sub>0--t} \<subseteq> U (X t\<^sub>0)\<close> 
-      by (auto simp: closed_segment_eq_real_ivl)
+    hence "\<forall>r\<in>{t\<^sub>0--\<tau>}. G (X r)" and "{t\<^sub>0--\<tau>} \<subseteq> U (X t\<^sub>0)"
+      using Ghyp ivl closed_segment_closed_segment_subset ivl by blast+ 
     hence "\<mu> (X \<tau>) \<noteq> \<nu> (X \<tau>)"
-      using dI tHyp xivp(2) ivp_solsI[of X f U "X t\<^sub>0", OF xivp(1) _ xivp(3) t0Hyp]
-      unfolding diff_inv_eq by force
+      using dI xivp ivp_solsI[of X f, OF _ _ ends_in_segment(1)[of t\<^sub>0 \<tau>]] 
+      unfolding diff_inv_eq
+      by (metis (full_types) closed_segment_commute ends_in_segment(2) \<open>\<tau> \<in> {t\<^sub>0--t}\<close> 
+          has_vderiv_on_subset order_less_irrefl subset_closed_segment)
     hence "False"
       using \<open>\<mu> (X \<tau>) = \<nu> (X \<tau>)\<close> by blast}
   ultimately show "\<nu> (X t) < \<mu> (X t)"
     by fastforce
 qed
 
-lemma diff_inv_conj_rule [diff_inv_rules]:
-  assumes "diff_inv I\<^sub>1 f U S t\<^sub>0 G"
-    and "diff_inv I\<^sub>2 f U S t\<^sub>0 G"
-  shows "diff_inv (\<lambda>s. I\<^sub>1 s \<and> I\<^sub>2 s) f U S t\<^sub>0 G"
+lemma diff_inv_conjI [diff_inv_rules]:
+  assumes "diff_inv I\<^sub>1 f U t\<^sub>0 G"
+    and "diff_inv I\<^sub>2 f U t\<^sub>0 G"
+  shows "diff_inv (\<lambda>s. I\<^sub>1 s \<and> I\<^sub>2 s) f U t\<^sub>0 G"
   using assms unfolding diff_inv_def by auto
 
-lemma diff_inv_disj_rule [diff_inv_rules]:
-  assumes "diff_inv I\<^sub>1 f U S t\<^sub>0 G"
-    and "diff_inv I\<^sub>2 f U S t\<^sub>0 G"
-  shows "diff_inv (\<lambda>s. I\<^sub>1 s \<or> I\<^sub>2 s) f U S t\<^sub>0 G"
+lemma diff_inv_disjI [diff_inv_rules]:
+  assumes "diff_inv I\<^sub>1 f U t\<^sub>0 G"
+    and "diff_inv I\<^sub>2 f U t\<^sub>0 G"
+  shows "diff_inv (\<lambda>s. I\<^sub>1 s \<or> I\<^sub>2 s) f U t\<^sub>0 G"
   using assms unfolding diff_inv_def by auto
 
 
+subsection \<open> Picard-Lindeloef \<close>
+
+text\<open> A locale with the assumptions of Picard-Lindeloef's theorem. It extends 
+@{term "ll_on_open_it"} by providing an initial time @{term "t\<^sub>0 \<in> T"}.\<close>
+
+locale picard_lindeloef =
+  fixes f::"real \<Rightarrow> ('a::{heine_borel,banach}) \<Rightarrow> 'a" and T::"real set" and S::"'a set" and t\<^sub>0::real
+  assumes open_domain: "open T" "open S"
+    and interval_time: "is_interval T"
+    and init_time: "t\<^sub>0 \<in> T"
+    and cont_vec_field: "\<forall>s \<in> S. continuous_on T (\<lambda>t. f t s)"
+    and lipschitz_vec_field: "local_lipschitz T S f"
+begin
+
+sublocale ll_on_open_it T f S t\<^sub>0
+  by (unfold_locales) (auto simp: cont_vec_field lipschitz_vec_field interval_time open_domain) 
+
+lemma ll_on_open: "ll_on_open T f S"
+  using local.general.ll_on_open_axioms .
+
+lemmas subintervalI = closed_segment_subset_domain
+   and init_time_ex_ivl = existence_ivl_initial_time[OF init_time]
+   and flow_at_init[simp] = general.flow_initial_time[OF init_time]
+                               
+abbreviation "ex_ivl s \<equiv> existence_ivl t\<^sub>0 s"
+
+lemma flow_has_vderiv_on_ex_ivl:
+  assumes "s \<in> S"
+  shows "D flow t\<^sub>0 s = (\<lambda>t. f t (flow t\<^sub>0 s t)) on ex_ivl s"
+  using flow_usolves_ode[OF init_time \<open>s \<in> S\<close>] 
+  unfolding usolves_ode_from_def solves_ode_def by blast
+
+lemma flow_funcset_ex_ivl:
+  assumes "s \<in> S"
+  shows "flow t\<^sub>0 s \<in> ex_ivl s \<rightarrow> S"
+  using flow_usolves_ode[OF init_time \<open>s \<in> S\<close>] 
+  unfolding usolves_ode_from_def solves_ode_def by blast
+
+lemma flow_in_ivp_sols_ex_ivl:
+  assumes "s \<in> S"
+  shows "flow t\<^sub>0 s \<in> Sols f (ex_ivl s) t\<^sub>0 s"
+  using flow_has_vderiv_on_ex_ivl[OF assms] 
+  by (auto intro: ivp_solsI simp: init_time assms)
+
+lemma csols_eq: "csols t\<^sub>0 s = {(X, t). t \<in> T \<and>  X \<in> Sols f {t\<^sub>0--t} t\<^sub>0 s \<and> X \<in> {t\<^sub>0--t} \<rightarrow> S}"
+  unfolding ivp_sols_def csols_def solves_ode_def 
+  using closed_segment_subset_domain init_time by auto
+
+lemma subset_ex_ivlI:
+  "Y\<^sub>1 \<in> {t\<^sub>0--t} \<rightarrow> S \<Longrightarrow> Y\<^sub>1 \<in> Sols f T t\<^sub>0 s \<Longrightarrow> {t\<^sub>0--t} \<subseteq> T \<Longrightarrow> A \<subseteq> {t\<^sub>0--t} \<Longrightarrow> A \<subseteq> ex_ivl s"
+  apply(clarsimp simp: existence_ivl_def)
+  apply(subgoal_tac "t\<^sub>0 \<in> T", clarsimp simp: csols_eq)
+   apply(rule_tac x=Y\<^sub>1 in exI, rule_tac x=t in exI, safe, force)
+  by (rule in_ivp_sols_subset[OF ends_in_segment(1)], auto)
+
+lemma unique_solution: \<comment> \<open> proved for a subset of T for general applications \<close>
+  assumes "s \<in> S" and "t\<^sub>0 \<in> U" and "t \<in> U" 
+    and "is_interval U" and "U \<subseteq> ex_ivl s" 
+    and xivp: "D Y\<^sub>1 = (\<lambda>t. f t (Y\<^sub>1 t)) on U" "Y\<^sub>1 t\<^sub>0 = s" "Y\<^sub>1 \<in> U \<rightarrow> S"
+    and yivp: "D Y\<^sub>2 = (\<lambda>t. f t (Y\<^sub>2 t)) on U" "Y\<^sub>2 t\<^sub>0 = s" "Y\<^sub>2 \<in> U \<rightarrow> S"
+  shows "Y\<^sub>1 t = Y\<^sub>2 t"
+proof-
+  have "t\<^sub>0 \<in> T"
+    using assms existence_ivl_subset by auto
+  have key: "(flow t\<^sub>0 s usolves_ode f from t\<^sub>0) (ex_ivl s) S"
+    using flow_usolves_ode[OF \<open>t\<^sub>0 \<in> T\<close> \<open>s \<in> S\<close>] .
+  hence "\<forall>t\<in>U. Y\<^sub>1 t = flow t\<^sub>0 s t"
+    unfolding usolves_ode_from_def solves_ode_def apply safe
+    by (erule_tac x=Y\<^sub>1 in allE, erule_tac x=U in allE, auto simp: assms)
+  also have "\<forall>t\<in>U. Y\<^sub>2 t = flow t\<^sub>0 s t"
+    using key unfolding usolves_ode_from_def solves_ode_def apply safe
+    by (erule_tac x=Y\<^sub>2 in allE, erule_tac x=U in allE, auto simp: assms)
+  ultimately show "Y\<^sub>1 t = Y\<^sub>2 t"
+    using assms by auto
+qed
+
+text \<open>Applications of lemma @{text "unique_solution"}: \<close>
+
+lemma unique_solution_closed_ivl:
+  assumes xivp: "D X = (\<lambda>t. f t (X t)) on {t\<^sub>0--t}" "X t\<^sub>0 = s" "X \<in> {t\<^sub>0--t} \<rightarrow> S" and "t \<in> T"
+    and yivp: "D Y = (\<lambda>t. f t (Y t)) on {t\<^sub>0--t}" "Y t\<^sub>0 = s" "Y \<in> {t\<^sub>0--t} \<rightarrow> S" and "s \<in> S" 
+  shows "X t = Y t"
+  apply(rule unique_solution[OF \<open>s \<in> S\<close>, of "{t\<^sub>0--t}"], simp_all add: assms)
+  apply(unfold existence_ivl_def csols_eq ivp_sols_def, clarsimp)
+  using xivp \<open>t \<in> T\<close> by blast
+
+lemma solution_eq_flow:
+  assumes xivp: "D X = (\<lambda>t. f t (X t)) on ex_ivl s" "X t\<^sub>0 = s" "X \<in> ex_ivl s \<rightarrow> S" 
+    and "t \<in> ex_ivl s" and "s \<in> S" 
+  shows "X t = flow t\<^sub>0 s t"
+  apply(rule unique_solution[OF \<open>s \<in> S\<close> init_time_ex_ivl \<open>t \<in> ex_ivl s\<close>])
+  using flow_has_vderiv_on_ex_ivl flow_funcset_ex_ivl \<open>s \<in> S\<close> by (auto simp: assms)
+
+(*
+lemma ivp_unique_solution:
+  assumes "s \<in> S" and ivl: "is_interval (U s)" and "U s \<subseteq> T" and "t \<in> U s" 
+    and ivp1: "Y\<^sub>1 \<in> Sols f U S t\<^sub>0 s" and ivp2: "Y\<^sub>2 \<in> Sols f U S t\<^sub>0 s"
+  shows "Y\<^sub>1 t = Y\<^sub>2 t"
+proof(rule unique_solution[OF \<open>s \<in> S\<close>, of "{t\<^sub>0--t}"], simp_all)
+  have "t\<^sub>0 \<in> U s"
+    using ivp_solsD[OF ivp1] by auto
+  hence obs0: "{t\<^sub>0--t} \<subseteq> U s"
+    using closed_segment_subset_interval[OF ivl] \<open>t \<in> U s\<close> by blast
+  moreover have obs1: "Y\<^sub>1 \<in> Sols f (\<lambda>s. {t\<^sub>0--t}) S t\<^sub>0 s"
+    by (rule in_ivp_sols_subset[OF _ calculation(1) ivp1], simp)
+  moreover have obs2: "Y\<^sub>2 \<in> Sols f (\<lambda>s. {t\<^sub>0--t}) S t\<^sub>0 s"
+    by (rule in_ivp_sols_subset[OF _ calculation(1) ivp2], simp)
+  ultimately show "{t\<^sub>0--t} \<subseteq> ex_ivl s"
+    apply(unfold existence_ivl_def csols_eq, clarsimp)
+    apply(rule_tac x=Y\<^sub>1 in exI, rule_tac x=t in exI)
+    using \<open>t \<in> U s\<close> and \<open>U s \<subseteq> T\<close> by force
+  show "D Y\<^sub>1 = (\<lambda>t. f t (Y\<^sub>1 t)) on {t\<^sub>0--t}"
+    by (rule ivp_solsD[OF in_ivp_sols_subset[OF _ _ ivp1]], simp_all add: obs0)
+  show "D Y\<^sub>2 = (\<lambda>t. f t (Y\<^sub>2 t)) on {t\<^sub>0--t}"
+    by (rule ivp_solsD[OF in_ivp_sols_subset[OF _ _ ivp2]], simp_all add: obs0)
+  show "Y\<^sub>1 t\<^sub>0 = s" and "Y\<^sub>2 t\<^sub>0 = s"
+    using ivp_solsD[OF ivp1] ivp_solsD[OF ivp2] by auto
+  show "Y\<^sub>1 \<in> {t\<^sub>0--t} \<rightarrow> S" and "Y\<^sub>2 \<in> {t\<^sub>0--t} \<rightarrow> S"
+    using ivp_solsD[OF obs1] ivp_solsD[OF obs2] by auto
+qed*)
+
+lemma g_orbital_orbit:
+  assumes "s \<in> S" and ivl: "is_interval (U s)" and "U s \<subseteq> T"
+    and ivp: "Y \<in> Sols f (U s) t\<^sub>0 s"
+  shows "g_orbital f G U t\<^sub>0 s = g_orbit G (U s) t\<^sub>0 Y"
+proof(rule set_eqI2)
+  have eq1: "\<forall>Z \<in> Sols f (U s) t\<^sub>0 s. \<forall>t\<in>U s. Z t = Y t"
+    by (clarsimp, rule ivp_unique_solution[OF assms(1,2,3) _ _ ivp], auto)
+  have "g_orbital f G U t\<^sub>0 s \<subseteq> g_orbit G (U s) t\<^sub>0 Y"
+  proof
+    fix x assume "x \<in> g_orbital f G U t\<^sub>0 s"
+    then obtain Z and t where z_def: "x = Z t \<and> {t\<^sub>0--t} \<subseteq> U s \<and> (\<forall>\<tau>\<in>{t\<^sub>0--t}. G (Z \<tau>))" 
+      and ivp: "Z \<in> Sols f {t\<^sub>0--t} t\<^sub>0 s"
+      unfolding g_orbital_eq by auto
+    hence "t\<^sub>0 \<in> U s"
+      by auto
+    hence "\<forall>\<tau>\<in>{t\<^sub>0--t}. Z \<tau> = Y \<tau>"
+      using z_def apply clarsimp
+      thm ivp[unfolded ivp_sols_def, simplified] unique_solution[OF assms(1)]
+      by (rule ivp_unique_solution[OF assms(1,2,3) _ _ ivp], auto)
+    thus "x \<in> g_orbit Y G (U s)"
+      using z_def eq1 unfolding g_orbit_eq by simp metis
+  qed
+  moreover have "g_orbit G (U s) t\<^sub>0 Y \<subseteq> g_orbital f G U t\<^sub>0 s"
+    apply(unfold g_orbital_eq g_orbit_def ivp_sols_def, clarsimp)
+    apply(rule_tac x=t in exI, rule_tac x=Y in exI)
+    using ivp_solsD[OF ivp] ivl \<open>t\<^sub>0 \<in> U s\<close> apply auto
+  ultimately show ?thesis
+    by blast
+qed
+
+end
+
+lemma local_lipschitz_add: 
+  fixes f1 f2 :: "real \<Rightarrow> 'a::banach \<Rightarrow> 'a"
+  assumes "local_lipschitz T S f1"
+      and "local_lipschitz T S f2" 
+    shows "local_lipschitz T S (\<lambda>t s. f1 t s + f2 t s)"
+proof(unfold local_lipschitz_def, clarsimp)
+  fix s and t assume "s \<in> S" and "t \<in> T"
+  obtain \<epsilon>\<^sub>1 L1 where "\<epsilon>\<^sub>1 > 0" and L1: "\<And>\<tau>. \<tau>\<in>cball t \<epsilon>\<^sub>1 \<inter> T \<Longrightarrow> L1-lipschitz_on (cball s \<epsilon>\<^sub>1 \<inter> S) (f1 \<tau>)"
+    using local_lipschitzE[OF assms(1) \<open>t \<in> T\<close> \<open>s \<in> S\<close>] by blast
+  obtain \<epsilon>\<^sub>2 L2 where "\<epsilon>\<^sub>2 > 0" and L2: "\<And>\<tau>. \<tau>\<in>cball t \<epsilon>\<^sub>2 \<inter> T \<Longrightarrow> L2-lipschitz_on (cball s \<epsilon>\<^sub>2 \<inter> S) (f2 \<tau>)"
+    using local_lipschitzE[OF assms(2) \<open>t \<in> T\<close> \<open>s \<in> S\<close>] by blast
+  have ballH: "cball s (min \<epsilon>\<^sub>1 \<epsilon>\<^sub>2) \<inter> S \<subseteq> cball s \<epsilon>\<^sub>1 \<inter> S" "cball s (min \<epsilon>\<^sub>1 \<epsilon>\<^sub>2) \<inter> S \<subseteq> cball s \<epsilon>\<^sub>2 \<inter> S"
+    by auto
+  have obs1: "\<forall>\<tau>\<in>cball t \<epsilon>\<^sub>1 \<inter> T. L1-lipschitz_on (cball s (min \<epsilon>\<^sub>1 \<epsilon>\<^sub>2) \<inter> S) (f1 \<tau>)"
+    using lipschitz_on_subset[OF L1 ballH(1)] by blast
+  also have obs2: "\<forall>\<tau>\<in>cball t \<epsilon>\<^sub>2 \<inter> T. L2-lipschitz_on (cball s (min \<epsilon>\<^sub>1 \<epsilon>\<^sub>2) \<inter> S) (f2 \<tau>)"
+    using lipschitz_on_subset[OF L2 ballH(2)] by blast
+  ultimately have "\<forall>\<tau>\<in>cball t (min \<epsilon>\<^sub>1 \<epsilon>\<^sub>2) \<inter> T. 
+    (L1 + L2)-lipschitz_on (cball s (min \<epsilon>\<^sub>1 \<epsilon>\<^sub>2) \<inter> S) (\<lambda>s. f1 \<tau> s + f2 \<tau> s)"
+    using lipschitz_on_add by fastforce
+  thus "\<exists>u>0. \<exists>L. \<forall>t\<in>cball t u \<inter> T. L-lipschitz_on (cball s u \<inter> S) (\<lambda>s. f1 t s + f2 t s)"
+    apply(rule_tac x="min \<epsilon>\<^sub>1 \<epsilon>\<^sub>2" in exI)
+    using \<open>\<epsilon>\<^sub>1 > 0\<close> \<open>\<epsilon>\<^sub>2 > 0\<close> by force
+qed
+
+lemma picard_lindeloef_add: "picard_lindeloef f1 T S t\<^sub>0 \<Longrightarrow> picard_lindeloef f2 T S t\<^sub>0 \<Longrightarrow> 
+  picard_lindeloef (\<lambda>t s. f1 t s + f2 t s) T S t\<^sub>0"
+  unfolding picard_lindeloef_def apply(clarsimp, rule conjI)
+  using continuous_on_add apply fastforce
+  using local_lipschitz_add by blast
+
+lemma picard_lindeloef_constant: "picard_lindeloef (\<lambda>t s. c) UNIV UNIV t\<^sub>0"
+  apply(unfold_locales, simp_all add: local_lipschitz_def lipschitz_on_def, clarsimp)
+  by (rule_tac x=1 in exI, clarsimp, rule_tac x="1/2" in exI, simp)
+
+
+subsection \<open> Flows for ODEs \<close>
+
+text\<open> A locale designed for verification of hybrid systems. The user can select the interval 
+of existence and the defining flow equation via the variables @{term "T"} and @{term "\<phi>"}.\<close>
+
+locale local_flow = picard_lindeloef "(\<lambda> t. f)" T S 0 
+  for f::"'a::{heine_borel,banach} \<Rightarrow> 'a" and T S L +
+  fixes \<phi> :: "real \<Rightarrow> 'a \<Rightarrow> 'a"
+  assumes ivp:
+    "\<And> t s. t \<in> T \<Longrightarrow> s \<in> S \<Longrightarrow> D (\<lambda>t. \<phi> t s) = (\<lambda>t. f (\<phi> t s)) on {0--t}"
+    "\<And> s. s \<in> S \<Longrightarrow> \<phi> 0 s = s"
+    "\<And> t s. t \<in> T \<Longrightarrow> s \<in> S \<Longrightarrow> (\<lambda>t. \<phi> t s) \<in> {0--t} \<rightarrow> S"
+begin
+
+lemma in_ivp_sols_ivl: 
+  assumes "t \<in> T" "s \<in> S"
+  shows "(\<lambda>t. \<phi> t s) \<in> Sols (\<lambda>t. f) {0--t} 0 s"
+  apply(rule ivp_solsI)
+  using ivp assms by auto
+
+lemma eq_solution_ivl:
+  assumes xivp: "D X = (\<lambda>t. f (X t)) on {0--t}" "X 0 = s" "X \<in> {0--t} \<rightarrow> S" 
+    and indom: "t \<in> T" "s \<in> S"
+  shows "X t = \<phi> t s"
+  apply(rule unique_solution_closed_ivl[OF xivp \<open>t \<in> T\<close>])
+  using \<open>s \<in> S\<close> ivp indom by auto
+
+lemma ex_ivl_eq:
+  assumes "s \<in> S"
+  shows "ex_ivl s = T"
+  using existence_ivl_subset[of s] apply safe
+  unfolding existence_ivl_def csols_eq
+  using in_ivp_sols_ivl[OF _ assms] ivp(3) apply auto
+  sorry
+
+lemma has_derivative_on_open1: 
+  assumes  "t > 0" "t \<in> T" "s \<in> S"
+  obtains B where "t \<in> B" and "open B" and "B \<subseteq> T"
+    and "D (\<lambda>\<tau>. \<phi> \<tau> s) \<mapsto> (\<lambda>\<tau>. \<tau> *\<^sub>R f (\<phi> t s)) at t within B" 
+proof-
+  obtain r::real where rHyp: "r > 0" "ball t r \<subseteq> T"
+    using open_contains_ball_eq open_domain(1) \<open>t \<in> T\<close> by blast
+  moreover have "t + r/2 > 0"
+    using \<open>r > 0\<close> \<open>t > 0\<close> by auto
+  moreover have "{0--t} \<subseteq> T" 
+    using subintervalI[OF init_time \<open>t \<in> T\<close>] .
+  ultimately have subs: "{0<--<t + r/2} \<subseteq> T"
+    unfolding abs_le_eq abs_le_eq real_ivl_eqs[OF \<open>t > 0\<close>] real_ivl_eqs[OF \<open>t + r/2 > 0\<close>] 
+    by clarify (case_tac "t < x", simp_all add: cball_def ball_def dist_norm subset_eq field_simps)
+  have "t + r/2 \<in> T"
+    using rHyp unfolding real_ivl_eqs[OF rHyp(1)] by (simp add: subset_eq)
+  hence "{0--t + r/2} \<subseteq> T"
+    using subintervalI[OF init_time] by blast
+  hence "(D (\<lambda>t. \<phi> t s) = (\<lambda>t. f (\<phi> t s)) on {0--(t + r/2)})"
+    using ivp(1)[OF _ \<open>s \<in> S\<close>] by auto
+  hence vderiv: "(D (\<lambda>t. \<phi> t s) = (\<lambda>t. f (\<phi> t s)) on {0<--<t + r/2})"
+    apply(rule has_vderiv_on_subset)
+    unfolding real_ivl_eqs[OF \<open>t + r/2 > 0\<close>] by auto
+  have "t \<in> {0<--<t + r/2}"
+    unfolding real_ivl_eqs[OF \<open>t + r/2 > 0\<close>] using rHyp \<open>t > 0\<close> by simp
+  moreover have "D (\<lambda>\<tau>. \<phi> \<tau> s) \<mapsto> (\<lambda>\<tau>. \<tau> *\<^sub>R f (\<phi> t s)) (at t within {0<--<t + r/2})"
+    using vderiv calculation unfolding has_vderiv_on_def has_vector_derivative_def by blast
+  moreover have "open {0<--<t + r/2}"
+    unfolding real_ivl_eqs[OF \<open>t + r/2 > 0\<close>] by simp
+  ultimately show ?thesis
+    using subs that by blast
+qed
+
+lemma has_derivative_on_open2: 
+  assumes "t < 0" "t \<in> T" "s \<in> S"
+  obtains B where "t \<in> B" and "open B" and "B \<subseteq> T"
+    and "D (\<lambda>\<tau>. \<phi> \<tau> s) \<mapsto> (\<lambda>\<tau>. \<tau> *\<^sub>R f (\<phi> t s)) at t within B" 
+proof-
+  obtain r::real where rHyp: "r > 0" "ball t r \<subseteq> T"
+    using open_contains_ball_eq open_domain(1) \<open>t \<in> T\<close> by blast
+  moreover have "t - r/2 < 0"
+    using \<open>r > 0\<close> \<open>t < 0\<close> by auto
+  moreover have "{0--t} \<subseteq> T" 
+    using subintervalI[OF init_time \<open>t \<in> T\<close>] .
+  ultimately have subs: "{0<--<t - r/2} \<subseteq> T"
+    unfolding open_segment_eq_real_ivl closed_segment_eq_real_ivl
+      real_ivl_eqs[OF rHyp(1)] by(auto simp: subset_eq)
+  have "t - r/2 \<in> T"
+    using rHyp unfolding real_ivl_eqs by (simp add: subset_eq)
+  hence "{0--t - r/2} \<subseteq> T"
+    using subintervalI[OF init_time] by blast
+  hence "(D (\<lambda>t. \<phi> t s) = (\<lambda>t. f (\<phi> t s)) on {0--(t - r/2)})"
+    using ivp(1)[OF _ \<open>s \<in> S\<close>] by auto
+  hence vderiv: "(D (\<lambda>t. \<phi> t s) = (\<lambda>t. f (\<phi> t s)) on {0<--<t - r/2})"
+    apply(rule has_vderiv_on_subset)
+    unfolding open_segment_eq_real_ivl closed_segment_eq_real_ivl by auto
+  have "t \<in> {0<--<t - r/2}"
+    unfolding open_segment_eq_real_ivl using rHyp \<open>t < 0\<close> by simp
+  moreover have "D (\<lambda>\<tau>. \<phi> \<tau> s) \<mapsto> (\<lambda>\<tau>. \<tau> *\<^sub>R f (\<phi> t s)) (at t within {0<--<t - r/2})"
+    using vderiv calculation unfolding has_vderiv_on_def has_vector_derivative_def by blast
+  moreover have "open {0<--<t - r/2}"
+    unfolding open_segment_eq_real_ivl by simp
+  ultimately show ?thesis
+    using subs that by blast
+qed
+
+lemma has_derivative_on_open3: 
+  assumes "s \<in> S"
+  obtains B where "0 \<in> B" and "open B" and "B \<subseteq> T"
+    and "D (\<lambda>\<tau>. \<phi> \<tau> s) \<mapsto> (\<lambda>\<tau>. \<tau> *\<^sub>R f (\<phi> 0 s)) at 0 within B" 
+proof-
+  obtain r::real where rHyp: "r > 0" "ball 0 r \<subseteq> T"
+    using open_contains_ball_eq open_domain(1) init_time by blast
+  hence "r/2 \<in> T" "-r/2 \<in> T" "r/2 > 0"
+    unfolding real_ivl_eqs by auto
+  hence subs: "{0--r/2} \<subseteq> T" "{0--(-r/2)} \<subseteq> T"
+    using subintervalI[OF init_time] by auto
+  hence "(D (\<lambda>t. \<phi> t s) = (\<lambda>t. f (\<phi> t s)) on {0--r/2})"
+    "(D (\<lambda>t. \<phi> t s) = (\<lambda>t. f (\<phi> t s)) on {0--(-r/2)})"
+    using ivp(1)[OF _ \<open>s \<in> S\<close>] by auto
+  also have "{0--r/2} = {0--r/2} \<union> closure {0--r/2} \<inter> closure {0--(-r/2)}"
+    "{0--(-r/2)} = {0--(-r/2)} \<union> closure {0--r/2} \<inter> closure {0--(-r/2)}"
+    unfolding closed_segment_eq_real_ivl \<open>r/2 > 0\<close> by auto
+  ultimately have vderivs:
+    "(D (\<lambda>t. \<phi> t s) = (\<lambda>t. f (\<phi> t s)) on {0--r/2} \<union> closure {0--r/2} \<inter> closure {0--(-r/2)})"
+    "(D (\<lambda>t. \<phi> t s) = (\<lambda>t. f (\<phi> t s)) on {0--(-r/2)} \<union> closure {0--r/2} \<inter> closure {0--(-r/2)})"
+    unfolding closed_segment_eq_real_ivl \<open>r/2 > 0\<close> by auto
+  have obs: "0 \<in> {-r/2<--<r/2}"
+    unfolding open_segment_eq_real_ivl using \<open>r/2 > 0\<close> by auto
+  have union: "{-r/2--r/2} = {0--r/2} \<union> {0--(-r/2)}"
+    unfolding closed_segment_eq_real_ivl by auto
+  hence "(D (\<lambda>t. \<phi> t s) = (\<lambda>t. f (\<phi> t s)) on {-r/2--r/2})"
+    using has_vderiv_on_union[OF vderivs] by simp
+  hence "(D (\<lambda>t. \<phi> t s) = (\<lambda>t. f (\<phi> t s)) on {-r/2<--<r/2})"
+    using has_vderiv_on_subset[OF _ segment_open_subset_closed[of "-r/2" "r/2"]] by auto
+  hence "D (\<lambda>\<tau>. \<phi> \<tau> s) \<mapsto> (\<lambda>\<tau>. \<tau> *\<^sub>R f (\<phi> 0 s)) (at 0 within {-r/2<--<r/2})"
+    unfolding has_vderiv_on_def has_vector_derivative_def using obs by blast
+  moreover have "open {-r/2<--<r/2}"
+    unfolding open_segment_eq_real_ivl by simp
+  moreover have "{-r/2<--<r/2} \<subseteq> T"
+    using subs union segment_open_subset_closed by blast 
+  ultimately show ?thesis
+    using obs that by blast
+qed
+
+lemma has_derivative_on_open: 
+  assumes "t \<in> T" "s \<in> S"
+  obtains B where "t \<in> B" and "open B" and "B \<subseteq> T"
+    and "D (\<lambda>\<tau>. \<phi> \<tau> s) \<mapsto> (\<lambda>\<tau>. \<tau> *\<^sub>R f (\<phi> t s)) at t within B" 
+  apply(subgoal_tac "t < 0 \<or> t = 0 \<or> t > 0")
+  using has_derivative_on_open1[OF _ assms] has_derivative_on_open2[OF _ assms]
+    has_derivative_on_open3[OF \<open>s \<in> S\<close>] by blast force
+
+lemma in_domain:
+  assumes "s \<in> S"
+  shows "(\<lambda>t. \<phi> t s) \<in> T \<rightarrow> S"
+  using ivp(3)[OF _ assms] by blast
+
+lemma has_vderiv_on_domain:
+  assumes "s \<in> S"
+  shows "D (\<lambda>t. \<phi> t s) = (\<lambda>t. f (\<phi> t s)) on T"
+proof(unfold has_vderiv_on_def has_vector_derivative_def, clarsimp)
+  fix t assume "t \<in> T"
+  then obtain B where "t \<in> B" and "open B" and "B \<subseteq> T" 
+    and Dhyp: "D (\<lambda>t. \<phi> t s) \<mapsto> (\<lambda>\<tau>. \<tau> *\<^sub>R f (\<phi> t s)) at t within B"
+    using assms has_derivative_on_open[OF \<open>t \<in> T\<close>] by blast
+  hence "t \<in> interior B"
+    using interior_eq by auto
+  thus "D (\<lambda>t. \<phi> t s) \<mapsto> (\<lambda>\<tau>. \<tau> *\<^sub>R f (\<phi> t s)) at t within T"
+    using has_derivative_at_within_mono[OF _ \<open>B \<subseteq> T\<close> Dhyp] by blast
+qed
+
+lemma in_ivp_sols: 
+  assumes "s \<in> S" and "0 \<in> U s" and "U s \<subseteq> T"
+  shows "(\<lambda>t. \<phi> t s) \<in> Sols (\<lambda>t. f) U S 0 s"
+  apply(rule in_ivp_sols_subset[OF _ _ ivp_solsI, of _ _ _ "\<lambda>s. T"])
+  using  ivp(2)[OF \<open>s \<in> S\<close>] has_vderiv_on_domain[OF \<open>s \<in> S\<close>] 
+    in_domain[OF \<open>s \<in> S\<close>] assms by auto
+
+lemma eq_solution:
+  assumes "s \<in> S" and "is_interval (U s)" and "U s \<subseteq> T" and "t \<in> U s"
+    and xivp: "X \<in> Sols (\<lambda>t. f) U S 0 s"
+  shows "X t = \<phi> t s"
+  apply(rule ivp_unique_solution[OF assms], rule in_ivp_sols)
+  by (simp_all add: ivp_solsD(4)[OF xivp] assms)
+
+lemma ivp_sols_collapse: 
+  assumes "T = UNIV" and "s \<in> S"
+  shows "Sols (\<lambda>t. f) (\<lambda>s. T) S 0 s = {(\<lambda>t. \<phi> t s)}"
+  apply (safe, simp_all add: fun_eq_iff, clarsimp)
+   apply(rule eq_solution[of _ "\<lambda>s. T"]; simp add: assms)
+  by (rule in_ivp_sols; simp add: assms)
+
+lemma additive_in_ivp_sols:
+  assumes "s \<in> S" and "\<P> (\<lambda>\<tau>. \<tau> + t) T \<subseteq> T"
+  shows "(\<lambda>\<tau>. \<phi> (\<tau> + t) s) \<in> Sols (\<lambda>t. f) (\<lambda>s. T) S 0 (\<phi> (0 + t) s)"
+  apply(rule ivp_solsI[OF vderiv_on_composeI])
+       apply(rule has_vderiv_on_subset[OF has_vderiv_on_domain])
+  using in_domain assms init_time by (auto intro!: poly_derivatives)
+
+lemma is_monoid_action:
+  assumes "s \<in> S" and "T = UNIV"
+  shows "\<phi> 0 s = s" and "\<phi> (t\<^sub>1 + t\<^sub>2) s = \<phi> t\<^sub>1 (\<phi> t\<^sub>2 s)"
+proof-
+  show "\<phi> 0 s = s"
+    using ivp assms by simp
+  have "\<phi> (0 + t\<^sub>2) s = \<phi> t\<^sub>2 s" 
+    by simp
+  also have "\<phi> (0 + t\<^sub>2) s \<in> S"
+    using in_domain assms by auto
+  ultimately show "\<phi> (t\<^sub>1 + t\<^sub>2) s = \<phi> t\<^sub>1 (\<phi> t\<^sub>2 s)"
+    using eq_solution[OF _ _ _ _ additive_in_ivp_sols] assms by auto
+qed
+
+lemma g_orbital_collapses: 
+  assumes "s \<in> S" and "is_interval (U s)" and "U s \<subseteq> T" and "0 \<in> U s"
+  shows "g_orbital (\<lambda>t. f) G U S 0 s = {\<phi> t s| t. t \<in> U s \<and> (\<forall>\<tau>\<in>down (U s) t. G (\<phi> \<tau> s))}"
+  apply (subst g_orbital_orbit[of _ _ "\<lambda>t. \<phi> t s"], simp_all add: assms g_orbit_eq)
+  by (rule in_ivp_sols, simp_all add: assms)
+
+definition orbit :: "'a \<Rightarrow> 'a set" ("\<gamma>\<^sup>\<phi>")
+  where "\<gamma>\<^sup>\<phi> s = g_orbital (\<lambda>t. f) (\<lambda>s. True) (\<lambda>s. T) S 0 s"
+
+lemma orbit_eq: 
+  assumes "s \<in> S"
+  shows "\<gamma>\<^sup>\<phi> s = {\<phi> t s| t. t \<in> T}"
+  apply(unfold orbit_def, subst g_orbital_collapses)
+  by (simp_all add: assms init_time interval_time)
+
+lemma true_g_orbit_eq:
+  assumes "s \<in> S"
+  shows "g_orbit (\<lambda>t. \<phi> t s) (\<lambda>s. True) T = \<gamma>\<^sup>\<phi> s"
+  unfolding g_orbit_eq orbit_eq[OF assms] by simp
+
+end
+
+lemma line_is_local_flow: 
+  "0 \<in> T \<Longrightarrow> is_interval T \<Longrightarrow> open T \<Longrightarrow> local_flow (\<lambda> s. c) T UNIV (\<lambda> t s. s + t *\<^sub>R c)"
+  apply(unfold_locales, simp_all add: local_lipschitz_def lipschitz_on_def, clarsimp)
+   apply(rule_tac x=1 in exI, clarsimp, rule_tac x="1/2" in exI, simp)
+  apply(rule_tac f'1="\<lambda> s. 0" and g'1="\<lambda> s. c" in has_vderiv_on_add[THEN has_vderiv_on_eq_rhs])
+    apply(rule derivative_intros, simp)+
+  by simp_all
+
+
+subsection \<open> Verification components \<close>
 
 type_synonym 'a pred = "'a \<Rightarrow> bool"
+type_synonym 's prog = "'s \<Rightarrow> 's set"
 
 definition fbox :: "('a \<Rightarrow> 'b set) \<Rightarrow> 'b pred \<Rightarrow> 'a pred" ("|_] _" [61,81] 82)
   where "|F] P = (\<lambda>s. (\<forall>s'. s' \<in> F s \<longrightarrow> P s'))"
@@ -470,12 +779,23 @@ lemma fbox_invariants:
     and "(\<lambda>s. I s \<or> J s) \<le> |F] (\<lambda>s. I s \<or> J s)"
   using assms unfolding fbox_def by auto
 
+subsection \<open> Verification of hybrid programs \<close>
+
+text \<open> Verification by providing evolution \<close>
+
+definition g_evol :: "(('a::real_vector) \<Rightarrow> 'b \<Rightarrow> 'b) \<Rightarrow> 'b pred \<Rightarrow> ('b \<Rightarrow> 'a set) \<Rightarrow> ('b \<Rightarrow> 'b set)" ("EVOL")
+  where "EVOL \<phi> G U = (\<lambda>s. g_orbit G (U s) 0 (\<lambda>t. \<phi> t s))"
+
+lemma fbox_g_evol[simp]: 
+  fixes \<phi> :: "('a::real_vector) \<Rightarrow> 'b \<Rightarrow> 'b"
+  shows "|EVOL \<phi> G U] Q = (\<lambda>s. (\<forall>t\<in>U s. (\<forall>\<tau>\<in>{0--t}. G (\<phi> \<tau> s)) \<longrightarrow> Q (\<phi> t s)))"
+  unfolding g_evol_def g_orbit_def fbox_def by auto
+
+text \<open> Verification by providing solutions \<close>
+
 lemma fbox_g_orbital: "|g_orbital f G U t\<^sub>0] Q = 
-  (\<lambda>s. \<forall>t. \<forall>X\<in>Sols f {t\<^sub>0--t} t\<^sub>0 s. {t\<^sub>0--t} \<subseteq> U (X t\<^sub>0) \<longrightarrow> (\<forall>\<tau>\<in>{t\<^sub>0--t}. G (X \<tau>)) \<longrightarrow> Q (X t))"
-  unfolding fbox_def g_orbital_eq apply(auto simp: fun_eq_iff)
-   apply(erule_tac x="X t" in allE, clarsimp, erule_tac x=t in allE)
-   apply(clarsimp simp: ivp_sols_def, erule_tac x=X in allE, force)
-  by (erule_tac x=t in allE, erule_tac x=X in ballE; clarsimp simp: ivp_sols_def)
+  (\<lambda>s. \<forall>t. \<forall>X\<in>Sols f {t\<^sub>0--t} t\<^sub>0 s. {t\<^sub>0--t} \<subseteq> U s \<longrightarrow> (\<forall>\<tau>\<in>{t\<^sub>0--t}. G (X \<tau>)) \<longrightarrow> Q (X t))"
+  unfolding fbox_def g_orbital_eq by (auto simp: fun_eq_iff)
 
 lemma fbox_g_orbital_ivl: "\<forall>s. is_interval (U s) \<and> t\<^sub>0 \<in> U s \<Longrightarrow> |g_orbital f G U t\<^sub>0] Q = 
   (\<lambda>s. \<forall>t\<in>U s. \<forall>X\<in>Sols f {t\<^sub>0--t} t\<^sub>0 s. (\<forall>\<tau>\<in>{t\<^sub>0--t}. G (X \<tau>)) \<longrightarrow> Q (X t))"
